
## Properties of Inverse Functions

In this post, I will be exploring some properties of inverse functions and the relationships between functions and their inverses.

First of all, I'd like to revisit how inverse functions are defined. If $f:A\to B$ is a bijective function, then its inverse $f^{-1}:B\to A$ is defined as the function with the property
$$f(x)=y\iff f^{-1}(y)=x, \forall x\in A,y \in B$$
and, as a direct consequence of this definition, $f^{-1}$ has the property
$$(f^{-1}\circ f)(x)=x, \forall x\in A$$
$$(f\circ f^{-1})(y)=y, \forall y\in B$$

However, since we will be dealing mostly with functions from reals to reals, it is more intuitive for us to state that if $f:\mathbb R\to\mathbb R$ is bijective, then
$$(f^{-1}\circ f)(x)=(f\circ f^{-1})(x)=x, \forall x\in \mathbb R$$

We can use this simple property to prove an interesting result about the relationship between the first derivative of $f$ and that of its inverse. Since
$$(f\circ f^{-1})(x)=x$$
Then, by differentiating both sides and using the chain rule,
$$(f'\circ f^{-1})(x)\cdot \frac{d}{dx}f^{-1}(x)=1$$
and so
$$\frac{d}{dx}f^{-1}(x)=\frac{1}{(f'\circ f^{-1})(x)}$$

We can find a corresponding property relating the antiderivative of $f$ to the antiderivative of its inverse. If $F$ is the antiderivative of $f$, then we can evaluate
$$\int f^{-1}(x)dx$$
in terms of $F$ and $f^{-1}$. By making the substitution $x=f(u)$, we have
$$=\int uf'(u)du$$
and, by integration by parts, this is equal to
$$=uf(u)-\int f(u)du$$
$$=uf(u)-F(u)+C$$
and when we reverse our substitution, we get
$$=xf^{-1}(x)-(F\circ f^{-1})(x)+C$$
and so our final result is
$$\int f^{-1}(x)dx=xf^{-1}(x)-(F\circ f^{-1})(x)+C$$




