
## A summary of functional iteration

*2017 Nov 4*

In this post, I will pose a few functional-iteration puzzles, rederive some useful iteration formulas, and discover a few new ones. All of the most important formulas are colored green, so that they will stand out.

> Find a formula for the *nth* iterate of each of the following functions:
$$f_1(x)=x^{\ln(x)}$$
$$f_2(x)=x^{\ln(x)+2}$$
$$f_3(x)=\ln(e^x+1)$$
$$f_4(x)=\ln(e^x+1)+1$$
$$f_5(x)=\frac{\ln(e^x+1)+\ln(e^x-1)}{2}$$
$$f_6(x)=x+\ln(e^x+2)$$

Before getting into any formulas or puzzles, I must remind the reader of the most important principle of functional iteration. If $g,h$ are functions, then
$$\color{green}{(g^{-1}\circ h\circ g)^{\circ n}=g^{-1}\circ h^{\circ n}\circ g}$$
This fundamental property of function composition allows us to reduce difficult problems to easier ones. For example, consider the function
$$f(x)=\alpha x+\beta$$
In a previous post, I iterated this by forming a geometric series - however, it can be done in a much simpler way. Notice that we can rearrange this to obtain
$$f(x)=\alpha \bigg(x+\frac{\beta}{\alpha-1}\bigg)-\frac{\beta}{\alpha-1}$$
for $\alpha\ne 1$. Then, if we define $g$ and $h$ as
$$g(x)=x+\frac{\beta}{\alpha-1}$$
$$h(x)=\alpha x$$
we can write
$$f(x)=(g^{-1}\circ h\circ g)(x)$$
and so
$$f^{\circ n}(x)=(g^{-1}\circ h\circ g)^{\circ n}(x)$$
$$f^{\circ n}(x)=(g^{-1}\circ h^{\circ n}\circ g)(x)$$
Now we have reduced this problem to finding the *nth* iterate of $h$, which we can instantly say is
$$h^{\circ n}(x)=\alpha^n x$$
And now we may say that
$$\begin{align}
f^{\circ n}(x) & = (g^{-1}\circ h^{\circ n}\circ g)(x) \\
 & = h^{\circ n}\bigg(x+\frac{\beta}{\alpha-1}\bigg)-\frac{\beta}{\alpha-1} \\
 & = \alpha^n\bigg(x+\frac{\beta}{\alpha-1}\bigg)-\frac{\beta}{\alpha-1} \\
 & = \alpha^n x+\frac{\alpha^n -1}{\alpha-1}\beta \\
\end{align}$$
and our final formula is:
$$\color{green}{f(x)=\alpha x+\beta \implies f^{\circ n}(x)=\alpha^n x+\frac{\alpha^n -1}{\alpha-1}\beta}$$
Using the same method, one may derive this analogous formula:
$$\color{green}{f(x)=\beta x^\alpha \implies f^{\circ n}(x)=\beta^{\frac{\alpha^n -1}{\alpha-1}}x^{\alpha^n}}$$

Now I will move on to iterating a quadratic. Unfortunately, it seems that only a few specific types of quadratics can be effectively iterated. One rather obvious class of quadratic is the set of quadratics in the form
$$f(x)=\frac{(\alpha x+\beta)^2}{\alpha}-\frac{\beta}{\alpha}$$
Notice that we may let $g(x)=ax+b$ and $h(x)=x^2$ to discover that
$$f^{\circ n}(x)=\frac{1}{\alpha}(\alpha x+\beta)^{2^n}-\frac{\beta}{\alpha}$$
Before we make this into a final formula, I would like to rearrange $f$ so that $f$ is written in standard quadratic form:
$$\begin{align}
f(x) &= \frac{(\alpha x+\beta)^2}{\alpha}-\frac{\beta}{\alpha} \\
 &= \frac{\alpha^2 x^2+2\alpha\beta x+\beta ^2 }{\alpha}-\frac{\beta}{\alpha} \\
 &= \alpha x+2\beta x+\frac{\beta ^2-\beta}{\alpha} \\
\end{align}$$
and, if we let $2\beta=\gamma$,
$$f(x)=\alpha x+\gamma x+\frac{\gamma ^2-\gamma}{4\alpha}$$
and
$$f^{\circ n}(x)=\frac{1}{\alpha}\bigg(\alpha x+\frac{\gamma}{2}\bigg)^{2^n}-\frac{\gamma}{2\alpha}$$
and so we are ready for our third formula:
$$\color{green}{f(x)=\alpha x+\gamma x+\frac{\gamma ^2-\gamma}{4\alpha}\implies f^{\circ n}(x)=\frac{1}{\alpha}\bigg(\alpha x+\frac{\gamma}{2}\bigg)^{2^n}-\frac{\gamma}{2\alpha}}$$

There is one more special type of quadratic that can be readily evaluated, and it originates from the double-angle formula of the cosine function:
$$\cos 2\theta=2\cos^2\theta-1$$
This allows us to say that
$$\cos (2\arccos x)=2x^2-1$$
for all $x$ with $|x|\le 1$. Do you recognize this as being in the form $g^{-1}\circ h\circ g$? If we let
$$f(x)=2x^2-1$$
$$g(x)=\arccos x$$
$$h(x)=2x$$
then we may readily state that
$$f^{\circ n}(x)=\cos(2^n\arccos x)$$
However, this can be generalized. If we instead let
$$f(x)=\alpha x^2+\beta x+\frac{\beta^2-2\beta-8}{4\alpha}=\frac{2}{\alpha}\cos\bigg(2\arccos\frac{2\alpha x+\beta}{4}\bigg)-\frac{\beta}{2\alpha}$$
with $g(x)=\arccos \frac{2\alpha x+\beta}{4}$ and $h(x)=2x$, then we may say that
$$\color{green}{f(x)=\alpha x^2+\beta x+\frac{\beta^2-2\beta-8}{4\alpha}\implies f^{\circ n}(x)=\frac{2}{\alpha}\cos\bigg(2^n\arccos\frac{2\alpha x+\beta}{4}\bigg)-\frac{\beta}{2\alpha}}$$
However, this only works for a very small domain, since the inverse cosine function is defined only for inputs between $-1$ and $1$. But this is an easy fix - as a result of Euler's famous formula linking the trigonometric functions to the complex exponential function,
$$\cosh(ix)=\cos(x)$$
and
$$-i\operatorname{arccosh}(x)=\arccos(x)$$
which means that
$$\alpha x^2+\beta x+\frac{\beta^2-2\beta-8}{4\alpha}=\frac{2}{\alpha}\cosh\bigg(2\operatorname{arccosh}\frac{2\alpha x+\beta}{4}\bigg)-\frac{\beta}{2\alpha}$$
and, because of the symmetry of a parabola, we may extend this property past the domain of the inverse hyperbolic cosine function:
$$\alpha x^2+\beta x+\frac{\beta^2-2\beta-8}{4\alpha}=\frac{2}{\alpha}\cosh\bigg(2\operatorname{arccosh}\bigg|\frac{2\alpha x+\beta}{4}\bigg|\bigg)-\frac{\beta}{2\alpha}$$
and so, at last, we may complete our pair of iteration formulas for this type of quadratic:
$$\color{green}{f(x)=\alpha x^2+\beta x+\frac{\beta^2-2\beta-8}{4\alpha}\implies f^{\circ n}(x)=\frac{2}{\alpha}\cosh\bigg(2^n\operatorname{arccosh}\bigg|\frac{2\alpha x+\beta}{4}\bigg|\bigg)-\frac{\beta}{2\alpha}}$$

The two choices of $g$ and $h$ that I used to iterate these quadratics can also be used for other polynomials. For example, if
$$f(x)=x^3+3x^2+3x$$
then we may write
$$f(x)=(x+1)^3-1$$
and so, by choosing $g(x)=x+1$ and $h(x)=x^3$,
$$f^{\circ n}(x)=(x+1)^{3^n}-1$$
The method using multiple-angle formulas of the cosine function can also be used for other polynomials. In fact, polynomials that are in such a form are called *chebyshev polynomials*. The *nth* chebyshev polynomial is defined as the unique polynomial solution to the functional equation
$$T_n(\cos\theta)=\cos(n\theta),\forall \theta$$

This wonderful method can also be used to find iteration formulas for certain rational functions. For example, consider a rational function in the form
$$f(x)=\frac{x}{\alpha x+\beta}$$
This rational function can be rewritten as
$$f(x)=\frac{1/\alpha}{\beta\frac{1/\alpha}{x}+1}$$
and so, if we let $g(x)=\frac{1/\alpha}{x}$ and $h(x)=\beta x+1$ and use our second formula,
$$f^{\circ n}(x)=\frac{1/\alpha}{\beta^n\frac{1/\alpha}{x}+\frac{\beta^n-1}{\beta-1}}$$
or
$$f^{\circ n}(x)=\frac{x(\beta-1)}{\beta^n(\beta-1)+\alpha(\beta^n-1)x}$$
and so we have another useful formula:
$$\color{green}{f(x)=\frac{x}{\alpha x+\beta}\implies f^{\circ n}(x)=\frac{x(\beta-1)}{\beta^n(\beta-1)+\alpha(\beta^n-1)x}}$$
We can use this special case to write an iteration formula for *any* first degree rational function. Suppose that
$$f(x)=\frac{\alpha x+\beta}{x+\gamma}$$
Then let us define the function $F$ as
$$F(x)=f(x+k)-k=\frac{(\alpha-k)x-k^2+(\alpha-\gamma)k+\beta}{x+k+\gamma}$$
for some $k$. This is a helpful substitution to make, since $F(x)=f(x+k)-k$ implies that
$$F^{\circ n}(x)=f^{\circ n}(x+k)-k$$
and so if we find an iteration formula for $F$, we may find one for $f$ as well. If we want $F$ to be in the form that we already know how to iterate, we can choose $k$ such that 
$$-k^2+(\alpha-\gamma)k+\beta=0$$
or, by the quadratic formula,
$$k=\frac{\alpha-\gamma\pm \sqrt{(\alpha-\gamma)^2+4b}}{2}$$
So, if we set $k$ equal to that value, we have
$$F(x)=\frac{(\alpha-k)x}{x+k+\gamma}$$
or
$$F(x)=\frac{x}{\frac{1}{\alpha-k}x+\frac{\gamma+k}{\alpha-k}}$$
Now it is in the form that we already know how to iterate, and using the previous formula, we may immediately write
$$F^{\circ n}(x)=\frac{x\big(\frac{\gamma +k}{\alpha -k}-1\big)}{\big(\frac{\gamma +k}{\alpha -k}\big)^n\big(\frac{\gamma +k}{\alpha -k}-1\big)+\frac{1}{\alpha-k}\big(\big(\frac{\gamma+k}{\alpha-k}\big)^n-1\big)x}$$
and, since $F^{\circ n}(x)=f^{\circ n}(x+k)-k$, we have that $f^{\circ n}(x)=F^{\circ n}(x-k)+k$, and so
$$f^{\circ n}(x)=\frac{(x-k)\big(\frac{\gamma +k}{\alpha -k}-1\big)}{\big(\frac{\gamma +k}{\alpha -k}\big)^n\big(\frac{\gamma +k}{\alpha -k}-1\big)+\frac{1}{\alpha-k}\big(\big(\frac{\gamma+k}{\alpha-k}\big)^n-1\big)(x-k)}+k$$
and so we have our final formula:
$$\color{green}{f(x)=\frac{\alpha x+\beta}{x+\gamma}\implies f^{\circ n}(x)=\frac{(x-k)\big(\frac{\gamma +k}{\alpha -k}-1\big)}{\big(\frac{\gamma +k}{\alpha -k}\big)^n\big(\frac{\gamma +k}{\alpha -k}-1\big)+\frac{1}{\alpha-k}\big(\big(\frac{\gamma+k}{\alpha-k}\big)^n-1\big)(x-k)}+k}$$
$$\color{green}{\text{where}\space\space\space\space k=\frac{\alpha-\gamma\pm \sqrt{(\alpha-\gamma)^2+4b}}{2}}$$

Now I will solve the puzzles that I posed at the beginning of the post. The first function was
$$f_1(x)=x^{\ln(x)}$$
To iterate this, one must notice that
$$x^{\ln(x)}=e^{\ln(x)^2}$$
and if we choose $g(x)=\ln(x)$ and $h(x)=x^2$, we have
$$f_1^{\circ n}(x)=e^{\ln(x)^{2^n}}$$

Now for the second function:
$$f_2(x)=x^{\ln(x)+2}$$
We may rewrite $f_2$ as
$$f_2(x)=e^{\ln(x)^2+2\ln(x)}$$
or
$$f_2(x)=e^{(\ln(x)+1)^2-1}$$
and so, if we let $g(x)=\ln(x)+1$ and $h(x)=x^2$, we have
$$f_2^{\circ n}(x)=e^{(\ln(x)+1)^{2^n}-1}$$

The third function is
$$f_3(x)=\ln(e^x+1)$$
This problem is not difficult - in fact, I solved it in an earlier post. By letting $g(x)=e^x$ and $h(x)=x+1$, we have
The third function is
$$f_3^{\circ n}(x)=\ln(e^x+n)$$

The fourth function is very similar:
$$f_4(x)=\ln(e^x+1)+1$$
It can be rewritten as
$$f_4(x)=\ln(e\cdot e^x+e)$$
and if we let $g(x)=e^x$ and $h(x)=ex+e$ and use our second formula, we have
$$f_4^{\circ n}(x)=\ln\bigg(e^n\cdot e^x+\frac{e^n-1}{e-1}e\bigg)$$
or
$$f_4^{\circ n}(x)=\ln\bigg(e^{x+n-1}+\frac{e^n-1}{e-1}\bigg)+1$$

Now the fifth function:
$$f_5(x)=\frac{\ln(e^x+1)+\ln(e^x-1)}{2}$$
This can be rewritten as
$$f_5(x)=\frac{\ln((e^x+1)(e^x-1))}{2}=\frac{\ln(e^{2x}-1)}{2}$$
and so, by letting $g(x)=e^{2x}$ and $h(x)=x-1$,
$$f_5^{\circ n}(x)=\frac{\ln(e^{2x}-n)}{2}$$

Now for the sixth and final function:
$$f_6(x)=x+\ln(e^x+2)$$
This can be written as
$$f_6(x)=\ln(e^{2x}+2e^x)=\ln((e^x+1)^2-1)$$
and so, if we let $g(x)=e^x+1$ and $h(x)=x^2$,
$$f_6^{\circ n}(x)=\ln((e^x+1)^{2^n}-1)$$

That's all for now! Let me remind you that my solutions to each of these problems were *not* instantaneous - the solutions you are seeing are polished, thought-out solutions. When trying these problems for the first time, my work was nowhere near as quick and tidy.


