
## Reciprocal-Fibonacci Series

*2018 Jan 30*

>Evaluate the following infinite series, where $F_n$ is the *nth* fibonacci number with $F_1=F_2=1$:
$$\sum_{k=1}^\infty \frac{(-1)^{k+1}}{F_k F_{k+5}}=\space\space\space ?$$
$$\sum_{k=1}^\infty \frac{1}{F_k F_{k+6}}=\space\space\space ?$$
$$\sum_{k=1}^\infty \frac{(-1)^{k+1}}{F_{5k-1}F_{5k+4}}=\space\space\space ?$$
$$\sum_{k=1}^\infty \frac{1}{F_{10k}F_{10k+10}}=\space\space\space ?$$

To evaluate these series, consider the functions $\Phi_n(x)$ defined as
$$\Phi_n(x):=\sum_{k=1}^\infty \frac{x^{k+1}}{F_k F_{k+n}}$$
where $F_k$ are the Fibonacci numbers, with $F_1=F_2=1$. In this post, I shall endeavour to evaluate a few particular value of $\Phi_n(x)$, establish a few of its functional equations to make computation easier, and use the functional equations to evaluate related sums.

First, recall the following well-known identities:
$$F_{k+n}=F_k F_{n-1}+F_{k+1}F_n$$
$$F_k^2-F_{k+1}F_{k-1}=(-1)^{k+1}$$
which I will use frequently throughout the post.

I shall begin by computing $\Phi_1(-1)$ and $\Phi_2(1)$, which are both straightforward telescoping sums:
$$\begin{align}
\Phi_1(-1) &= \sum_{k=1}^\infty \frac{(-1)^{k+1}}{F_k F_{k+1}}\\
&= 1+\sum_{k=2}^\infty \frac{F_k^2-F_{k+1}F_{k-1}}{F_k F_{k+1}}\\
&= 1-\sum_{k=2}^\infty \frac{F_{k-1}}{F_{k}}-\frac{F_k}{F_{k+1}}\\
&= 1-1+\lim_{k\to\infty} \frac{F_k}{F_{k+1}}\\
&= \phi^{-1}\\
\end{align}$$
Where $\phi$ is the golden ratio $\frac{1+\sqrt 5}{2}$. Next, we have
$$\begin{align}
\Phi_2(1) &= \sum_{k=1}^\infty \frac{1}{F_k F_{k+2}}\\
&= \sum_{k=1}^\infty \frac{1}{F_k F_{k+1}}-\frac{1}{F_{k+1}F_{k+2}}\\
&= 1+\lim_{k\to\infty} \frac{1}{F_{k+1}F_{k+2}}\\
&= 1\\
\end{align}$$

Now I will establish a recurrence relation that allows one to compute additional values of $\Phi_n(x)$ using the two previously computed as initial conditions.

>**Theorem 1:**
$$\Phi_n(x)=\frac{\Phi_1(x)}{F_n}-\frac{F_{n-1}}{F_n}\frac{\Phi_{n-1}(x)}{x}+\frac{F_{n-1}x}{F_n^2}$$

**Proof:**

$$\begin{align}
\Phi_n(x) &=\sum_{k=1}^\infty \frac{x^{k+1}}{F_k F_{k+n}}\\
&=\sum_{k=1}^\infty \frac{x^{k+1}}{F_k (F_k F_{n-1}+F_{k+1}F_n)}\\
&=\sum_{k=1}^\infty \frac{x^{k+1}}{F_{k+1}F_n}\bigg(\frac{1}{F_k}-\frac{F_{n-1}}{F_{k+n}}\bigg)\\
&=\frac{\Phi_1(x)}{F_n}-\frac{F_{n-1}}{F_n}\sum_{k=1}^\infty \frac{x^{k+1}}{F_{k+1}F_{k+n}}\\
&=\frac{\Phi_1(x)}{F_n}+\frac{F_{n-1}}{F_n}\bigg(\frac{x}{F_n}-\sum_{k=1}^\infty \frac{x^{k}}{F_{k}F_{k+n-1}}\bigg)\\
&=\frac{\Phi_1(x)}{F_n}+\frac{F_{n-1}}{F_n}\bigg(\frac{x}{F_n}-\frac{\Phi_{n-1}(x)}{x}\bigg)\\
&= \frac{\Phi_1(x)}{F_n}-\frac{F_{n-1}}{F_n}\frac{\Phi_{n-1}(x)}{x}+\frac{F_{n-1}x}{F_n^2}\space\space\space\space\space\space\blacksquare\\
\end{align}$$

Through this formula, one may recursively calculate many values of $\Phi_n(1)$ and $\Phi_{n}(-1)$. For example, using $\Phi_1(-1)=\phi^{-1}$ as previously calculated,
$$\begin{align}
\Phi_2(-1) &=\frac{\Phi_1(-1)}{F_2}-\frac{F_1}{F_2}\frac{\Phi_1(-1)}{-1}+\frac{F_1 (-1)}{F_2^2}\\
&=2\Phi_1(-1)-1\\
&=2\phi^{-1}-1\\
\end{align}$$

and

$$\begin{align}
\Phi_3(-1) &=\frac{\Phi_1(-1)}{F_3}-\frac{F_2}{F_3}\frac{\Phi_2(-1)}{-1}+\frac{F_2 (-1)}{F_3^2}\\
&=\frac{\phi^{-1}}{2}+\frac{2\phi^{-1}-1}{2}-\frac{1}{4}\\
&=\frac{3\phi^{-1}}{2}-\frac{3}{4}\\
\end{align}$$

In fact, one may solve the recurrence relation to obtain the following:

>**Theorem 2:**
$$\Phi_n(x)=\frac{\Phi_1(x)}{F_n}\sum_{k=0}^{n-1} (-x)^{-k}-\frac{1}{F_n}\sum_{k=0}^{n-1}\frac{(-x)^{1-k}F_{n-k-1}}{F_{n-k}},\space\space\space n\ge 1$$

**Proof:** The base case of this formula - with $n=1$ - holds trivially, so I will now begin the induction step.

Suppose that
$$\Phi_m(x)=\frac{\Phi_1(x)}{F_m}\sum_{k=0}^{m-1} (-x)^{-k}-\frac{1}{F_m}\sum_{k=0}^{m-1}\frac{(-x)^{1-k}F_{m-k-1}}{F_{m-k}}$$
is true for some $m$. Then it follows that
$$-\frac{F_{m}}{F_{m+1} x}\Phi_m(x)=-\frac{\Phi_1(x)}{F_{m+1}x}\sum_{k=0}^{m-1} (-x)^{-k}+\frac{1}{F_{m+1} x}\sum_{k=0}^{m-1}\frac{(-x)^{1-k}F_{m-k-1}}{F_{m-k}}$$
$$-\frac{F_{m}}{F_{m+1} x}\Phi_m(x)=\frac{\Phi_1(x)}{F_{m+1}}\sum_{k=1}^{m} (-x)^{-k}-\frac{1}{F_{m+1}}\sum_{k=0}^{m-1}\frac{(-x)^{-k}F_{m-k-1}}{F_{m-k}}$$
$$\frac{\Phi_1(x)}{F_{m+1}}-\frac{F_{m}}{F_{m+1} x}\Phi_m(x)=\frac{\Phi_1(x)}{F_{m+1}}\sum_{k=0}^{m} (-x)^{-k}-\frac{1}{F_{m+1}}\sum_{k=0}^{m-1}\frac{(-x)^{-k}F_{m-k-1}}{F_{m-k}}$$
$$\frac{\Phi_1(x)}{F_{m+1}}-\frac{F_{m}}{F_{m+1} x}\Phi_m(x)+\frac{F_m x}{F_{m+1}^2}=\frac{\Phi_1(x)}{F_{m+1}}\sum_{k=0}^{m} (-x)^{-k}-\frac{1}{F_{m+1}}\sum_{k=0}^{m-1}\frac{(-x)^{-k}F_{m-k-1}}{F_{m-k}}+\frac{F_m x}{F_{m+1}^2}$$
$$\frac{\Phi_1(x)}{F_{m+1}}-\frac{F_{m}}{F_{m+1} x}\Phi_m(x)+\frac{F_m x}{F_{m+1}^2}=\frac{\Phi_1(x)}{F_{m+1}}\sum_{k=0}^{m} (-x)^{-k}-\frac{1}{F_{m+1}}\sum_{k=1}^{m}\frac{(-x)^{1-k}F_{m-k}}{F_{m-k+1}}+\frac{F_m x}{F_{m+1}^2}$$
$$\frac{\Phi_1(x)}{F_{m+1}}-\frac{F_{m}}{F_{m+1} x}\Phi_m(x)+\frac{F_m x}{F_{m+1}^2}=\frac{\Phi_1(x)}{F_{m+1}}\sum_{k=0}^{m} (-x)^{-k}-\frac{1}{F_{m+1}}\sum_{k=0}^{m}\frac{(-x)^{1-k}F_{m-k}}{F_{m-k+1}}$$
By Theorem 1, the LHS is equal to $\Phi_{m+1}(x)$, and so
$$\Phi_{m+1}(x)=\frac{\Phi_1(x)}{F_{m+1}}\sum_{k=0}^{m} (-x)^{-k}-\frac{1}{F_{m+1}}\sum_{k=0}^{m}\frac{(-x)^{1-k}F_{m-k}}{F_{m-k+1}}$$
Which shows that the formula holds for $m+1$ as well. Thus, by induction, it holds for all $n\ge 1$. $\blacksquare$

>**Corollary 1:**
$$\Phi_n(-1)=\frac{n\phi^{-1}}{F_n}-\frac{1}{F_n}\sum_{k=0}^{n-1} \frac{F_k}{F_{k+1}},\space\space\space n\ge 1$$

**Proof:** This follows directly from Theorem 2, since
$$\sum_{k=0}^{n-1} 1^{-k}=n$$
and since $\Phi_1(-1)=\phi^{-1}$. $\blacksquare$

> **Corollary 2:**
$$\Phi_{2n}(1)=\frac{1}{F_{2n}}\sum_{k=0}^{2n-1}\frac{(-1)^{k}F_{2n-k-1}}{F_{2n-k}},\space\space\space n\ge 1$$

**Proof:** This follows directly from Theorem 2, since 
$$\sum_{k=0}^{n-1} (-1)^{-k}=\begin{cases}
0 & \text{if n is even}\\
1 & \text{if n is odd}
\end{cases}$$

$\blacksquare$

> **Corollary 3:**
$$\Phi_{2n+1}(1)=\frac{\Phi_1(1)}{F_{2n+1}}+\frac{1}{F_{2n+1}}\sum_{k=1}^{n}\frac{1}{F_{2k}F_{2k+1}}, \space\space\space n\in\mathbb N, \space n\ge 1$$

**Proof:** This follows directly from Theorem 2, since 
$$\sum_{k=0}^{n-1} (-1)^{-k}=\begin{cases}
0 & \text{if n is even}\\
1 & \text{if n is odd}
\end{cases}$$

$\blacksquare$


Having derived these formulas, the answers to the first two proposed problems come easily:
$$\sum_{k=1}^\infty \frac{(-1)^{k+1}}{F_k F_{k+5}}=\phi^{-1}-\frac{83}{150}$$
$$\sum_{k=1}^\infty \frac{1}{F_k F_{k+6}}=\frac{143}{960}$$

I will now demonstrate how to use $\Phi_n(x)$ to evaluate a class of rather intimidating sums - sums in the form
$$\sum_{k=1}^\infty \frac{(-1)^{nk}}{F_{nk-m}F_{nk+n-m}},\space\space\text{with}\space\space\space 0\le m\le n-1$$
To evaluate these sums, I will make use of the properties of the complex roots of unity:
$$\omega_n := \cos \frac{2\pi}{n}+i\sin \frac{2\pi}{n}$$
I will now state two elementary properties (without proof) of the complex roots of unity that I will make use of later:
$$\sum_{p=0}^{n-1} (\omega_n^p)^k=
\begin{cases}
n & \text{if} \space\space\space n|k\\
0 & \text{else}
\end{cases}\tag 1$$
$$\sum_{k=0}^{n-1} (\omega_n^p)^k=
\begin{cases}
n & \text{if} \space\space\space \omega_n^p=1\\
0 & \text{else}\\
\end{cases}\tag 2$$

As a result,

>**Theorem 3:**
If
$$G(x):=\sum_{k=1}^\infty x^k a_k$$
Then
$$\sum_{p=0}^{n-1}(\omega_n^p)^m G(\omega_n^p)=n\sum_{k=1}^\infty a_{nk-m}$$

**Proof:** This theorem follows directly from properties (1) and (2) of the complex roots of unity. $\blacksquare$

Using the solution to the generalized recurrence and these identities, one may prove the following:

> **Theorem 4:**
$$\sum_{k=1}^\infty \frac{(-1)^{nk}}{F_{nk-m}F_{nk+n-m}}=(-1)^{m-1}\bigg[\frac{\phi^{-1}}{F_n}-\frac{F_{n-m-1}}{F_n F_{n-m}}\bigg],\space\space\space n\ge 2, \space\space 0\le m\le n-1$$

**Proof:** I shall divide this proof into two cases - one for even $n$, and one for odd $n$. We shall consider even $n$ first.

Suppose $n$ is even. I will begin with the following formula from Theorem 2:
$$\Phi_n(x)=\frac{\Phi_1(x)}{F_n}\sum_{k=0}^{n-1} (-x)^{-k}-\frac{1}{F_n}\sum_{k=0}^{n-1}\frac{(-x)^{1-k}F_{n-k-1}}{F_{n-k}}$$
Letting $x=\omega_n^p$, we have
$$\Phi_n(\omega_n^p)=\frac{\Phi_1(\omega_n^p)}{F_n}\sum_{k=0}^{n-1} (-\omega_n^p)^{-k}-\frac{1}{F_n}\sum_{k=0}^{n-1}\frac{(-\omega_n^p)^{1-k}F_{n-k-1}}{F_{n-k}}$$
$$(\omega_n^p)^{m-1}\Phi_n(\omega_n^p)=\frac{(-1)^{m-1}\Phi_1(\omega_n^p)}{F_n}\sum_{k=0}^{n-1} (-\omega_n^p)^{m-k-1}-\frac{(-1)^{m-1}}{F_n}\sum_{k=0}^{n-1}\frac{(-\omega_n^p)^{m-k}F_{n-k-1}}{F_{n-k}}$$
By property (2) of the roots of unity, when $\omega_n^p\ne -1$, this is equal to
$$(\omega_n^p)^{m-1}\Phi_n(\omega_n^p)=-\frac{(-1)^{m-1}}{F_n}\sum_{k=0}^{n-1}\frac{(-\omega_n^p)^{m-k}F_{n-k-1}}{F_{n-k}}$$
and when $\omega_n^p=-1$, it is equal to
$$(\omega_n^p)^{m-1}\Phi_n(\omega_n^p)=\frac{n(-1)^{m-1}\Phi_1(-1)}{F_n}-\frac{(-1)^{m-1}}{F_n}\sum_{k=0}^{n-1}\frac{(-\omega_n^p)^{m-k}F_{n-k-1}}{F_{n-k}}$$
$$(\omega_n^p)^{m-1}\Phi_n(\omega_n^p)=\frac{n(-1)^{m-1}\phi^{-1}}{F_n}-\frac{(-1)^{m-1}}{F_n}\sum_{k=0}^{n-1}\frac{(-\omega_n^p)^{m-k}F_{n-k-1}}{F_{n-k}}$$
This tells us that, since exactly one of the $\omega_n^p$ with $p$ between $0$ and $n-1$ is equal to $-1$,
$$\sum_{p=0}^{n-1}(\omega_n^p)^{m-1}\Phi_n(\omega_n^p)=\frac{n(-1)^{m-1}\phi^{-1}}{F_n}-\sum_{p=0}^{n-1}\frac{(-1)^{m-1}}{F_n}\sum_{k=0}^{n-1}\frac{(-\omega_n^p)^{m-k}F_{n-k-1}}{F_{n-k}}$$
$$\sum_{p=0}^{n-1}(\omega_n^p)^{m-1}\Phi_n(\omega_n^p)=\frac{n(-1)^{m-1}\phi^{-1}}{F_n}-\frac{(-1)^{m-1}}{F_n}\sum_{k=0}^{n-1}\bigg(\frac{F_{n-k-1}}{F_{n-k}}\sum_{p=0}^{n-1}(-\omega_n^p)^{m-k}\bigg)$$
Now note that since the sum $\sum_{p=0}^{n-1}(-\omega_n^p)^{m-k}$ cycles through the nth roots of unity, and since when $n$ is even, $\omega_n^p$ being a root of unity implies that $-\omega_n^p$ is also a root of unity, it is equal to the sum $\sum_{p=0}^{n-1}(\omega_n^p)^{m-k}$. Thus,
$$\sum_{p=0}^{n-1}(\omega_n^p)^{m-1}\Phi_n(\omega_n^p)=\frac{n(-1)^{m-1}\phi^{-1}}{F_n}-\frac{(-1)^{m-1}}{F_n}\sum_{k=0}^{n-1}\bigg(\frac{F_{n-k-1}}{F_{n-k}}\sum_{p=0}^{n-1}(\omega_n^p)^{m-k}\bigg)$$ 
and, by identity (1), this is
$$\sum_{p=0}^{n-1}(\omega_n^p)^{m-1}\Phi_n(\omega_n^p)=\frac{n(-1)^{m-1}\phi^{-1}}{F_n}-\frac{(-1)^{m-1}}{F_n}\sum_{k=0}^{n-1}\bigg(\frac{F_{n-k-1}}{F_{n-k}}\cdot\begin{cases}
n & \text{if} \space\space\space n|m-k\\
0 & \text{else}
\end{cases}\bigg)$$
Now, if one assumes that $0\le m\le n-1$, the only value of $k$ between $0$ and $n-1$ satisfying $n|m-k$ would be $k=m$. Thus, all terms of the sum are multiplied by zero except for the $k=m$ term, and all that remains is
$$\sum_{p=0}^{n-1}(\omega_n^p)^{m-1}\Phi_n(\omega_n^p)=\frac{n(-1)^{m-1}\phi^{-1}}{F_n}-\frac{n(-1)^{m-1}F_{n-m-1}}{F_nF_{n-m}}$$
Using Theorem 3, one may replace the LHS:
$$\sum_{k=1}^\infty \frac{n}{F_{nk-m}F_{nk+n-m}}=\frac{n(-1)^{m-1}\phi^{-1}}{F_n}-\frac{n(-1)^{m-1}F_{n-m-1}}{F_nF_{n-m}}$$
$$\sum_{k=1}^\infty \frac{1}{F_{nk-m}F_{nk+n-m}}=(-1)^{m-1}\bigg[\frac{\phi^{-1}}{F_n}-\frac{F_{n-m-1}}{F_nF_{n-m}}\bigg]$$
and, because $n$ is even, this is equivalent to
$$\sum_{k=1}^\infty \frac{(-1)^{nk}}{F_{nk-m}F_{nk+n-m}}=(-1)^{m-1}\bigg[\frac{\phi^{-1}}{F_n}-\frac{F_{n-m-1}}{F_nF_{n-m}}\bigg]$$
Which completes the proof for the case of even $n$.

Now suppose that $n$ is odd. Again, I will begin with the following formula from Theorem 2:
$$\Phi_n(x)=\frac{\Phi_1(x)}{F_n}\sum_{k=0}^{n-1} (-x)^{-k}-\frac{1}{F_n}\sum_{k=0}^{n-1}\frac{(-x)^{1-k}F_{n-k-1}}{F_{n-k}}$$
but this time, I will let $x=-\omega_n^p$, so that
$$\Phi_n(-\omega_n^p)=\frac{\Phi_1(-\omega_n^p)}{F_n}\sum_{k=0}^{n-1} (\omega_n^p)^{-k}-\frac{1}{F_n}\sum_{k=0}^{n-1}\frac{(\omega_n^p)^{1-k}F_{n-k-1}}{F_{n-k}}$$
$$(-\omega_n^p)^{m-1}\Phi_n(-\omega_n^p)=\frac{(-1)^{m-1}\Phi_1(-\omega_n^p)}{F_n}\sum_{k=0}^{n-1} (\omega_n^p)^{m-k-1}-\frac{(-1)^{m-1}}{F_n}\sum_{k=0}^{n-1}\frac{(\omega_n^p)^{m-k}F_{n-k-1}}{F_{n-k}}$$
By property (2) of the roots of unity, when $\omega_n^p\ne 1$, this is equal to
$$(-\omega_n^p)^{m-1}\Phi_n(-\omega_n^p)=-\frac{(-1)^{m-1}}{F_n}\sum_{k=0}^{n-1}\frac{(\omega_n^p)^{m-k}F_{n-k-1}}{F_{n-k}}$$
and when $\omega_n^p=1$, it is equal to
$$(-\omega_n^p)^{m-1}\Phi_n(-\omega_n^p)=\frac{n(-1)^{m-1}\Phi_1(-1)}{F_n}-\frac{(-1)^{m-1}}{F_n}\sum_{k=0}^{n-1}\frac{(\omega_n^p)^{m-k}F_{n-k-1}}{F_{n-k}}$$
$$(-\omega_n^p)^{m-1}\Phi_n(-\omega_n^p)=\frac{n(-1)^{m-1}\phi^{-1}}{F_n}-\frac{(-1)^{m-1}}{F_n}\sum_{k=0}^{n-1}\frac{(\omega_n^p)^{m-k}F_{n-k-1}}{F_{n-k}}$$
Because of this, one may say that
$$\sum_{p=0}^{n-1}(-\omega_n^p)^{m-1}\Phi_n(-\omega_n^p)=\frac{n(-1)^{m-1}\phi^{-1}}{F_n}-\sum_{p=0}^{n-1}\frac{(-1)^{m-1}}{F_n}\sum_{k=0}^{n-1}\frac{(\omega_n^p)^{m-k}F_{n-k-1}}{F_{n-k}}$$
$$\sum_{p=0}^{n-1}(-\omega_n^p)^{m-1}\Phi_n(-\omega_n^p)=\frac{n(-1)^{m-1}\phi^{-1}}{F_n}-\frac{(-1)^{m-1}}{F_n}\sum_{k=0}^{n-1}\bigg(\frac{F_{n-k-1}}{F_{n-k}}\sum_{p=0}^{n-1}(\omega_n^p)^{m-k} \bigg)$$
By property (1), this is
$$\sum_{p=0}^{n-1}(-\omega_n^p)^{m-1}\Phi_n(-\omega_n^p)=\frac{n(-1)^{m-1}\phi^{-1}}{F_n}-\frac{(-1)^{m-1}}{F_n}\sum_{k=0}^{n-1}\bigg(\frac{F_{n-k-1}}{F_{n-k}}\cdot
\begin{cases}
n & \text{if} \space\space\space n|m-k\\
0 & \text{else}
\end{cases}  \bigg)$$
If one assumes that $0\le m\le n-1$, the only term of the sum that does not vanish is the term for which $k=m$. Thus,
$$\sum_{p=0}^{n-1}(-\omega_n^p)^{m-1}\Phi_n(-\omega_n^p)=\frac{n(-1)^{m-1}\phi^{-1}}{F_n}-\frac{(-1)^{m-1}}{F_n}\frac{nF_{n-m-1}}{F_{n-m}}$$
$$\sum_{p=0}^{n-1}(-\omega_n^p)^{m-1}\Phi_n(-\omega_n^p)=(-1)^{m-1}\bigg[\frac{n\phi^{-1}}{F_n}-\frac{nF_{n-m-1}}{F_nF_{n-m}}\bigg]$$
By Theorem 3, the LHS can be replaced with an infinite series:
$$n\sum_{k=1}^\infty \frac{(-1)^{nk}}{F_{nk-m}F_{nk+n-m}}=(-1)^{m-1}\bigg[\frac{n\phi^{-1}}{F_n}-\frac{nF_{n-m-1}}{F_nF_{n-m}}\bigg]$$
and so, at last,
$$\sum_{k=1}^\infty \frac{(-1)^{nk}}{F_{nk-m}F_{nk+n-m}}=(-1)^{m-1}\bigg[\frac{\phi^{-1}}{F_n}-\frac{F_{n-m-1}}{F_nF_{n-m}}\bigg]$$
Which completes the proof for the case of odd $n$. Thus I have established that
$$\sum_{k=1}^\infty \frac{(-1)^{nk}}{F_{nk-m}F_{nk+n-m}}=(-1)^{m-1}\bigg[\frac{\phi^{-1}}{F_n}-\frac{F_{n-m-1}}{F_nF_{n-m}}\bigg],\space\space\space n\ge 2, \space\space 0\le m\le n-1 \space\space\space\blacksquare$$

With this formula, the third and fourth proposed problems may be solved readily:
$$\sum_{k=1}^\infty \frac{(-1)^{k+1}}{F_{5k-1}F_{5k+4}}= \frac{2}{15}-\frac{\phi^{-1}}{5}$$
$$\sum_{k=1}^\infty \frac{1}{F_{10k}F_{10k+10}}=\frac{\phi^{-1}}{55}-\frac{34}{3025}$$	



