
## Interesting Trigonometric Integrals

*2018 June 16*

**NOTE:** I will use a special notation during this post that may be unfamiliar to some. The symbol $\delta_{ij}$, a function of $i$ and $j$, is defined as $1$ if $i=j$ and $0$ otherwise... pretty simple, but handy since it allows one to avoid piecewise notation. 

**NOTE:** One more piece of helpful notation - the Iverson Bracket. If $A$ is some logical statement, then $[A]$ is equal to $1$ if $A$ is true and $0$ if $A$ is false. For example, $[2018\space\text{is odd}]=0$, and $\delta_{ij}=[i=j]$.
 
> $$\int_0^\pi \frac{\cos(5x)}{5-\cos(x)}dx$$
$$\int_0^\pi \frac{dx}{(5-4\cos(x))(5-4\cos(2x))}$$
$$\int_0^\infty \frac{1-\cos(2x)}{5-4\cos(2x)}\frac{dx}{x^2}$$
$$\int_0^\infty \ln(2-2\cos(x^2))dx$$

**WARNING:** Don't try to calculate the last integral in any nice closed form - I calculated it in terms of a fractional value of the Zeta function.

As with my last blog post, the integrals provided as "warm-ups" are only specific cases of more useful generalizations that I will derive during this post. Interestingly, some of these integrals involve a bit of number theory, which we will discover shortly...

Let us begin with the following integral, which I have not included in the warm-ups, but which is crucial in my derivation of many of them:
$$\int_0^\pi \cos(mx)\cos(nx)dx$$
...where $m$ and $n$ are positive integers. Using the following trigonometric identity:
$$\cos(\theta)\cos(\phi)=\frac{\cos(\theta+\phi)+\cos(\theta-\phi)}{2}$$
we can transform the integral into the following:
$$\int_0^\pi \frac{\cos((m+n)x)+\cos((m-n)x)}{2}dx$$
which easily evaluates to 
$$\frac{\sin((m+n)\pi)}{2m+2n}+\frac{\sin((m-n)\pi)}{2m-2n}$$
which vanishes for any positive integers $m,n$, since the sine of an integer multiple of $\pi$ is zero. However, this integral isn't valid for $m=n$, because the second term, in that case, is indeterminant. When $m=n$, the integral becomes instead
$$\int_0^\pi \frac{\cos((m+n)x)+\cos(0)}{2}dx$$
which evaluates to $\pi/2$. Thus, our original integral vanishes when $m\ne n$ and is equal to $\pi/2$ when $m=2$, giving us the following result:
$$\int_0^\pi \cos(mx)\cos(nx)dx=\frac{\pi}{2}\delta_{mn}$$
...a rather tame result on its own, but, in conjunction with some other trigonometric series and integral identities, it can lead to some fascinating ones.

To start us on this journey, I shall begin with a rather ordinary generating function identity. As we all know,
$$\sum_{n=0}^\infty x^n=\frac{1}{1-x}$$
By replacing $x$ with $ze^{i\theta}$, we have the following: 
$$\begin{align}
\sum_{n=0}^\infty (ze^{i\theta})^n
&=\frac{1}{1-ze^{i\theta}}\\
&=\frac{1}{1-z\cos\theta-iz\sin\theta}\\
&=\frac{1-z\cos\theta+iz\sin\theta}{(1-z\cos\theta-iz\sin\theta)(1-z\cos\theta+iz\sin\theta)}\\
&=\frac{1-z\cos\theta+iz\sin\theta}{(1-z\cos\theta)^2+z^2\sin^2\theta}\\
&=\frac{1-z\cos\theta+iz\sin\theta}{1-2z\cos\theta+z^2\cos^2\theta+z^2\sin^2\theta}\\
&=\frac{1-z\cos\theta+iz\sin\theta}{1-2z\cos\theta+z^2}\\
\end{align}$$
By equating real and imaginary parts, this demonstrates that
$$\sum_{n=0}^\infty z^n\cos(n\theta)=\frac{1-z\cos\theta}{1-2z\cos\theta+z^2}$$
$$\sum_{n=0}^\infty z^n\sin(n\theta)=\frac{z\sin\theta}{1-2z\cos\theta+z^2}$$

Now, let's consider what this means when applied to our integral. We know that
$$\int_0^\pi \cos(mx)\cos(nx)dx=\frac{\pi}{2}\delta_{mn}$$
Thus if $k$ is a positive integer, then
$$\int_0^\pi z^k\cos(mkx)\cos(nx)dx=\frac{\pi}{2}z^k\delta_{(mk)n}$$
By summing both sides from $k=0$ to $\infty$, we get the following:
$$\int_0^\pi \frac{1-z\cos(mx)}{1+z^2-2z\cos(mx)}\cos(nx)dx=\frac{\pi}{2}z^{n/m}[m|n]$$
...as long as $|z|<1$, to ensure convergence. By decomposing that ugly fraction in the integral, we get the following:
$$\frac{1}{2}\int_0^\pi \bigg(\frac{1-z^2}{1+z^2-2z\cos(mx)}+1\bigg)\cos(nx)dx=\frac{\pi}{2}z^{n/m}[m|n]$$
...and, recalling the assumption that $n$ is an integer, we have

$$\bbox[lightgray,5px]{
\int_0^\pi \frac{\cos(nx)}{1+z^2-2z\cos(mx)}dx=\frac{\pi z^{n/m}[m|n]}{1-z^2}
}$$

This formula holds for $m,n\in\mathbb Z^+$ and $|z|<1$. Using it, we can easily resolve our first warm-up problem by setting $n=5$, $m=1$, and $z=5-2\sqrt{6}$:

$$\bbox[lightgray,5px]{
\int_0^\pi \frac{\cos(5x)}{5-\cos(x)}dx=\frac{2\pi (5-2\sqrt{6})^6}{1-(5-2\sqrt 6)^2}
}$$

...but we can do even better! In fact, we can do yet another infinite series! Let's begin this time with the formula we just derived:

$$\int_0^\pi \frac{\cos(nx)}{1+z^2-2z\cos(mx)}dx=\frac{\pi z^{n/m}[m|n]}{1-z^2}$$

This time, we'll replace $n$ with $nk$, where $k$ is a positive integer. For convenience's sake, I'll also replace $z$ with $a$.

$$\int_0^\pi \frac{\cos(nkx)}{1+a^2-2a\cos(mx)}dx=\frac{\pi a^{nk/m}[m|nk]}{1-a^2}$$

Now multiply both sides by $b^k$, for some $b$ satisfying $|b|<1$:

$$\int_0^\pi \frac{b^k\cos(nkx)}{1+a^2-2a\cos(mx)}dx=b^k\frac{\pi a^{nk/m}[m|nk]}{1-a^2}$$

Finally (can you guess what to do now?) I will sum both sides from $k=0$ to $\infty$, resulting in

$$\int_0^\pi \frac{1}{1+a^2-2a\cos(mx)}\frac{1-b\cos(nx)}{1+b^2-2b\cos(nx)}dx=\sum_{k=0}^\infty b^k\frac{\pi a^{nk/m}[m|nk]}{1-a^2}$$

Now notice that $[m|nk]$ is equal to zero unless $k$ is a multiple of $m/\gcd(m,n)$, in which case it is equal to $1$. Thus, our series can be converted to

$$\sum_{k=0}^\infty b^{mk/\gcd(m,n)}\frac{\pi a^{nk/\gcd(m,n)}}{1-a^2}$$

which is just a geometric series, converging to

$$\frac{\pi}{(1-a^2)(1-a^{n/\gcd(m,n)}b^{m/\gcd(m,n)})}$$

and so we have

$$\int_0^\pi \frac{1}{1+a^2-2a\cos(mx)}\frac{1-b\cos(nx)}{1+b^2-2b\cos(nx)}dx=\frac{\pi}{(1-a^2)(1-a^{n/\gcd(m,n)}b^{m/\gcd(m,n)})}$$

using the same partial fraction decomposition as before, we end up with the following:
$$\int_0^\pi \frac{1}{1+a^2-2a\cos(mx)}\frac{1}{1+b^2-2b\cos(nx)}dx=\frac{2\pi}{(1-a^2)(1-b^2)(1-a^{n/\gcd(m,n)}b^{m/\gcd(m,n)})}-\frac{\pi}{(1-a^2)(1-b^2)}$$
or
$$\bbox[lightgray,5px]{
\int_0^\pi \frac{dx}{(1+a^2-2a\cos(mx))(1+b^2-2b\cos(nx))}=\pi\frac{1+a^{n/\gcd(m,n)}b^{m/\gcd(m,n)}}{(1-a^2)(1-b^2)(1-a^{n/\gcd(m,n)}b^{m/\gcd(m,n)})}
}$$

Letting $m=1$, $n=2$, and $a=b=1/2$ gives the answer to the second warm-up:

$$\bbox[lightgray,5px]{
\int_0^\pi \frac{dx}{(5-4\cos(x))(5-4\cos(2x))}=\frac{\pi}{7}
}$$

Now we will use the infinite series identity derived earlier to exploit an entirely different type of integral. Consider the well-known identity 
$$\int_0^\infty \frac{\sin(ax)}{x}dx=\frac{\pi}{2}$$
for any value of $a$. By antidifferentiating both sides with respect to $a$, we obtain the integral
$$\int_0^\infty \frac{1-\cos(ax)}{x^2}dx=\frac{\pi a}{2}+C$$
where $C$ is some constant. By setting $a=0$, we see that $C=0$, and so
$$\int_0^\infty \frac{1-\cos(ax)}{x^2}dx=\frac{\pi a}{2}$$
Then replace $a$ with $ak$ for some positive integer $k$, and multiply both sides by $z^k$, where $|z|\lt 1$. This gives us
$$\int_0^\infty \frac{z^k-z^k\cos(axk)}{x^2}dx=\frac{\pi a}{2}\cdot kz^k$$
Now, as before, we sum both sides from $k=1$ to $\infinity$, and use this series identity before on the LHS:
$$\sum_{n=0}^\infty z^n\cos(n\theta)=\frac{1-z\cos\theta}{1-2z\cos\theta+z^2}$$
and use the following well-known series identity on the RHS:
$$\sum_{k=1}^\infty kz^k=\frac{z}{(1-z)^2}$$
This gives us the following equality:
$$\int_0^\infty \bigg(\frac{1}{1-z}-\frac{1-z\cos(ax)}{1+z^2-2z\cos(ax)}\bigg)\frac{dx}{x^2}=\frac{\pi a}{2}\cdot \frac{z}{(1-z)^2}$$
$$\int_0^\infty \frac{z^2+z-(z^2+z)\cos(ax)}{1+z^2-2z\cos(ax)}\frac{dx}{x^2}=\frac{\pi a}{2}\cdot \frac{z}{(1-z)^2}$$
or, as our final result,
$$\bbox[lightgray,5px]{
\int_0^\infty \frac{1-\cos(ax)}{1+z^2-2z\cos(ax)}\frac{dx}{x^2}=\frac{\pi a}{2}\cdot \frac{1}{(1-z)^2(1+z)}
}$$
Plugging in $z=1/4$, we get the value of our third warm-up problem:
$$\bbox[lightgray,5px]{
\int_0^\infty \frac{1-\cos(2x)}{5-4\cos(2x)}\frac{dx}{x^2}=\frac{\pi}{3}
}$$
For the next warm-up integral, before I start to solve it, I'd like to show a picture of its graph. It is, of course, an improper integral, but over the interval $(0,\infty)$, not only does its integrand contain infinitely many singularities, but they occur more and more frequently, making it *very* improper (so improper that Wolfram Alpha can't even approximate it effectively), but still convergent.

<center>![Fig 1](/img/2018-6-16-Fig1.png)</center> 

To quickly derive the value of this integral, one can employ the integral identity
$$\int_0^\infty \cos(ax^2)dx=\frac{1}{2}\sqrt{\frac{\pi}{2a}}$$
and the well-known Fourier series
$$\sum_{k=1}^\infty \frac{\cos(kx)}{k}=-\frac{\ln(2-2\cos(x))}{2}$$
By replacing $a$ with $ak$ in the first integral and dividing both sides by $k$, one obtains
$$\int_0^\infty \frac{\cos(akx^2)}{k}dx=\frac{1}{2}\sqrt{\frac{\pi}{2a}}\frac{1}{k^{3/2}}$$
Then, summing from $k=1$ to $\infty$, one gets
$$\bbox[lightgray,5px]{
\int_0^\infty \ln(2-2\cos(ax^2))dx=-\sqrt{\frac{\pi}{2a}}\zeta(3/2)
}$$
By plugging in $a=1$, one gets the value of the fourth and final warm-up:
$$\bbox[lightgray,5px]{
\int_0^\infty \ln(2-2\cos(x^2))dx=-\sqrt{\frac{\pi}{2}}\zeta(3/2)
}$$
Now, before ending this blog post, I would like to show off an integral that I derived using trigonometric series. Using the Fourier Series that we employed for the previous series, and using the identity
$$\int_0^\pi \cos(mx)\cos(nx)dx=\frac{\pi}{2}\delta_{mn}$$
from earlier,along with various trigonometric identities, I managed to prove the following awesome identity for $m,n\in\mathbb Z$:
$$\bbox[lightgray,5px]{
\int_0^{\pi/2}\ln|\sin(mx)|\ln|\sin(nx)|dx=\frac{\pi^3}{24}\frac{\gcd^2(m,n)}{mn}+\frac{\pi\ln^2(2)}{2}
}$$

If you want, you can try it as well. And, to finish off the post, I propose the following exercise: see what integrals you can derive using trigonometric series and the following identity, derived in my post on the Residue Theorem:

$$\int_{-\infty}^\infty \frac{\cos(ax)}{x^2+1}dx=\pi e^{-|a|}$$





