
## The Gamma and Digamma functions

*2018 March 10*

Before I get into the definitions and the properties of these two functions, I must first introduce a new mathematical constant: the **Euler-Mascheroni** constant
$$\gamma\approx 0.57721566...$$
This constant is defined as follows:
$$\gamma := \lim_{n\to\infty} (H_n-\ln(n))$$
where $H_n$ are the harmonic numbers.

I will now establish an integral representation of the Euler-Mascheroni constant which will prove to be useful later on. Recall that the harmonic numbers $H_n$ are given by
$$H_n=\int_0^1 \frac{1-x^n}{1-x}dx=\int_0^1\frac{1-(1-x)^n}{x}dx$$
and recall that
$$\ln(n)=\int_{1/n}^1 \frac{dx}{x}$$
Recall also the value of the limit
$$\lim_{n\to\infty}\bigg(1+\frac{x}{n}\bigg)^n=e^x$$
which will come into play shortly.

By definition, we have
$$\begin{align}\gamma 
&= \lim_{n\to\infty} \bigg(\int_0^1\frac{1-(1-x)^n}{x}dx-\int_{1/n}^1 \frac{dx}{x}\bigg)\\
&= \lim_{n\to\infty} \bigg(\int_0^{1/n}\frac{1-(1-x)^n}{x}dx+\int_{1/n}^1\frac{1-(1-x)^n}{x}dx-\int_{1/n}^1 \frac{dx}{x}\bigg)\\
&= \lim_{n\to\infty} \bigg(\int_0^{1/n}\frac{1-(1-x)^n}{x}dx-\int_{1/n}^1\frac{(1-x)^n}{x}dx\bigg)\\
&= \lim_{n\to\infty} \bigg(\int_0^{1}\frac{1-(1-\frac{x}{n})^n}{x}dx-\int_{1}^n\frac{(1-\frac{x}{n})^n}{x}dx\bigg)\\
&= \lim_{n\to\infty} \bigg(\int_0^{1}\frac{1-e^{-x}}{x}dx-\int_{1}^n\frac{e^{-x}}{x}dx\bigg)\\
&= \int_0^{1}\frac{1-e^{-x}}{x}dx-\int_{1}^\infty \frac{e^{-x}}{x}dx\\
\end{align}$$

and so

$$\bbox[lightgray,5px]
{
\gamma=\int_0^{1}\frac{1-e^{-x}}{x}dx-\int_{1}^\infty \frac{e^{-x}}{x}dx
}$$

This is the integral representation that I was looking for! Now I will get into the definitions and properties of the gamma and digamma functions, and the Euler-Mascheroni constant will show up eventually - just wait.

In my [previous post](/post/85) about the Gamma and Lambert-W functions, I introduced the **Gamma function**, but did not explore its properties in much depth. Here is its definition:

$$\Gamma(z):=\int_0^\infty x^{z-1}e^{-x}dx$$

For positive integer $z$, it holds that
$$\Gamma(z)=(z-1)!$$
and, in general, the gamma function has the property
$$\Gamma(z+1)=z\Gamma(z)$$
which I demonstrated in my other post by integrating by parts. It also has the special value
$$\Gamma(1/2)=\sqrt{\pi}$$
which is the famed "Gaussian integral." 

Before moving on to the digamma function, I would like to prove the following property of the gamma function, relating it to the **Beta function** $\mathrm{B}(a,b)$:
$$\mathrm{B}(a,b):=\int_{0}^1 x^{a-1}(1-x)^{b-1}dx=\frac{\Gamma(a)\Gamma(b)}{\Gamma(a+b)}$$
Here is the proof:
$$\begin{align}
\Gamma(a)\Gamma(b)
&=\int_0^\infty \int_0^\infty x^{a-1}y^{b-1}e^{-x-y}dydx\\
&=4\int_0^\infty \int_0^\infty x^{2a-1}y^{2b-1}e^{-x^2-y^2}dydx\\
&=4\int_0^{\pi/2} \int_0^\infty (r\cos\theta)^{2a-1}(r\sin\theta)^{2b-1}e^{-r^2} rdrd\theta\\
&=4\int_0^{\pi/2} \int_0^\infty r^{2a+2b-1}\cos^{2a-1}(\theta)\sin^{2b-1}(\theta)e^{-r^2} drd\theta\\
&=2\int_0^{\pi/2} \int_0^\infty r^{a+b-1}\cos^{2a-1}(\theta)\sin^{2b-1}(\theta)e^{-r} drd\theta\\
&=2\bigg(\int_0^{\pi/2} \cos^{2a-1}(\theta)\sin^{2b-1}(\theta) d\theta\bigg) \bigg(\int_0^\infty r^{a+b-1}e^{-r}dr\bigg)\\
&=2\bigg(\int_0^{\pi/2} \cos^{2a-1}(\theta)\sin^{2b-1}(\theta) d\theta\bigg) \Gamma(a+b)\\
&=2\Gamma(a+b)\int_0^{1} \cos^{2a-1}(\arcsin x)\sin^{2b-1}(\arcsin x) \frac{dx}{\sqrt{1-x^2}}\\
&=2\Gamma(a+b)\int_0^{1} (1-x^2)^{a-1}x^{2b-1} dx\\
&=\Gamma(a+b)\int_0^{1} (1-x)^{a-1}x^{b-1} dx\\
&=\Gamma(a+b)\mathrm{B}(a,b)\\
\end{align}$$
and so
$$\Gamma(a)\Gamma(b)=\Gamma(a+b)\mathrm{B}(a,b)$$
and
$$\bbox[lightgray,5px]
{
\mathrm{B}(a,b)=\frac{\Gamma(a)\Gamma(b)}{\Gamma(a+b)}
}$$

This result can be used to prove Legendre's famous duplication formula for the Gamma Function, which expresses $\Gamma(2z)$ in terms of $\Gamma(z)$ and $\Gamma(z+1/2)$. Recall the definition of the Beta function:
$$\mathrm{B}(a,b):=\int_{0}^1 x^{a-1}(1-x)^{b-1}dx$$
By substituting $x\to x^2$ in the definite integral, this is equivalent to
$$\mathrm{B}(a,b)=2\int_{0}^1 x^{2a-1}(1-x^2)^{b-1}dx=\frac{\Gamma(a)\Gamma(b)}{\Gamma(a+b)}$$
Notice also that, by substituting $x\to \frac{1+x}{2}$ in the original integral, we have
$$\mathrm{B}(a,b)=\frac{1}{2}\int_{-1}^1 \bigg(\frac{1+x}{2}\bigg)^{a-1}\bigg(\frac{1-x}{2}\bigg)^{b-1}dx$$
and, as a consequence,
$$\begin{align}
\mathrm{B}(z,z)
&=\frac{1}{2}\int_{-1}^1 \bigg(\frac{1+x}{2}\bigg)^{z-1}\bigg(\frac{1-x}{2}\bigg)^{z-1}dx\\
&=\frac{1}{2^{2z-1}}\int_{-1}^1 (1+x)^{z-1} (1-x)^{z-1}dx\\
&=2^{1-2z}\int_{-1}^1 (1-x^2)^{z-1}dx\\
&=2^{1-2z}\cdot 2\int_{0}^1 (1-x^2)^{z-1}dx\\
&=2^{1-2z}\mathrm{B}(1/2,z)\\
\end{align}$$
Thus, we have
$$\mathrm{B}(z,z)=2^{1-2z}\mathrm{B}(1/2,z)$$
Now, by using the representation of the Beta function in terms of the Gamma function, we have
$$\frac{\Gamma(z)\Gamma(z)}{\Gamma(2z)}=\frac{2^{1-2z}\Gamma(1/2)\Gamma(z)}{\Gamma(z+1/2)}$$
which can be rearranged to obtain

$$\bbox[lightgray,5px]
{
\Gamma(2z)=\frac{2^{2z-1}\Gamma(z)\Gamma(z+1/2)}{\sqrt \pi}
}$$

which is the final form of the Gamma function's duplication formula.

Now I will introduce the **Digamma** function, defined as
$$\psi(z):=\frac{d}{dz}\ln \Gamma(z)=\frac{\Gamma'(z)}{\Gamma(z)}$$
I will start by calculating a few values of the digamma function - this is where the Euler-Mascheroni constant starts to appear. Since the Gamma function is defined as
$$\Gamma(z):=\int_0^\infty x^{z-1}e^{-x}dx$$
we have
$$\Gamma'(z)=\int_0^\infty x^{z-1}e^{-x}\ln(x)dx$$
and so
$$\psi(z)=\Gamma(z)\int_0^\infty x^{z-1}e^{-x}\ln(x)dx$$
Let us first endeavour to calculate the value of $\psi(1)$:
$$\psi(1)=\int_0^\infty e^{-x}\ln(x)dx$$
Using integration by parts, we have
$$\begin{align}
\psi(1)
&=\int_0^\infty e^{-x}\ln(x)dx\\
&=\int_0^1 e^{-x}\ln(x)dx+\int_1^\infty e^{-x}\ln(x)dx\\
&=\bigg[(1-e^{-x})\ln(x)\bigg]_0^1-\int_0^1 \frac{1-e^{-x}}{x}dx+\int_1^\infty e^{-x}\ln(x)dx\\
&=-\int_0^1 \frac{1-e^{-x}}{x}dx+\int_1^\infty e^{-x}\ln(x)dx\\
&=-\int_0^1 \frac{1-e^{-x}}{x}dx+\bigg[-e^{-x}\ln(x)\bigg]_1^\infty +\int_1^\infty \frac{e^{-x}}{x}dx\\
&=-\int_0^1 \frac{1-e^{-x}}{x}dx+\int_1^\infty \frac{e^{-x}}{x}dx\\
&=-\int_0^1 \frac{1-e^{-x}}{x}dx+\int_1^\infty \frac{e^{-x}}{x}dx\\
&=-\gamma\\
\end{align}$$

The last step in this equality is justified by the integral representation of $\gamma$ that we obtained earlier. Thus, we have
$$\psi(1)=-\gamma$$

We *could* go back and calculate $\psi(2)$, $\psi(3)$, and so on, but there's a shortcut to do this. Remember this recurrence for the gamma function that I mentioned earlier?
$$\Gamma(z+1)=z\Gamma(z)$$
By taking the natural logarithm of both sides, we have
$$\ln\Gamma(z+1)=\ln\Gamma(z)+\ln(z)$$
and by differentiating both sides with respect to $z$,
$$\psi(z+1)=\psi(z)+\frac{1}{z}$$
This tells us that, for any positive integer $n$,
$$\psi(n)=-\gamma+H_{n-1}$$
where $H_n$ are the harmonic numbers.

Observe the following. Since
$$\psi(z+1)-\psi(z)=\frac{1}{z}$$
as previously proven, we have that
$$\sum_{n=1}^N \frac{1}{n}=\psi(N+1)-\psi(1)=\psi(N+1)+\gamma$$
Furthermore, we also have that
$$\sum_{n=1}^N \frac{1}{n+z}=\psi(N+z+1)-\psi(z+1)$$
By subtracting these two equations, we have
$$\sum_{n=1}^N \frac{1}{n}-\frac{1}{n+z}=\psi(N+1)+\gamma-\psi(N+z+1)+\psi(z+1)$$
$$\sum_{n=1}^N \frac{1}{n}-\frac{1}{n+z}=(\psi(N+1)-\psi(N+z+1))+\psi(z+1)+\gamma$$
Now we let $N\to\infty$. As $N$ grows large, the term on the RHS inside of the parentheses approaches zero, and so we are left with
$$\sum_{n=1}^\infty \frac{1}{n}-\frac{1}{n+z}=\psi(z+1)+\gamma$$
Thus, we are left with the series representation for the digamma function:


$$\bbox[lightgray,5px]
{
\psi(z)=-\gamma+\sum_{n=0}^\infty\frac{1}{n+1}-\frac{1}{n+z}
}$$

Believe it or not, a *closed form* for the digamma function can be found for rational arguments. Though its derivation is a bit of a slog, I shall power through it for you. Using the series representation that we just derived, we have
$$\begin{align}
\psi(p/q)
&= -\gamma+\sum_{n=0}^\infty \frac{1}{n+1}-\frac{1}{n+\frac{p}{q}}\\
&= -\gamma+\sum_{n=0}^\infty \frac{1}{n+1}-\frac{q}{qn+p}\\
&= -\gamma+\sum_{n=0}^\infty\frac{1}{n+1}-\frac{q}{qn+p}\\
&= -\gamma+\lim_{x\to 1^-}\sum_{n=0}^\infty\frac{x^{n}}{n+1}-\frac{qx^{n}}{qn+p}\\
\end{align}$$
Now recall my [old blog post](/post/71) in which I devised a strategy for evaluating infinite series in the form
$$\sum_{n=0}^\infty \frac{x^{qn+p}}{qn+p}$$
for natural numbers $p$ and $q$. I will not explain the methods I use again in this post, so if you do not understand, I encourage you to go back to the old post. Using the complex roots of unity $\omega_n$, defined as
$$\omega_n:=e^{2\pi i/n}=\cos\frac{2\pi}{n}+i\sin\frac{2\pi}{n}$$
and using the fact that
$$\sum_{n=0}^\infty \frac{x^{n}}{n+1}=-\frac{\ln(1-x)}{x}$$
one can derive the following formula, for natural numbers $q$ and $p$ with $p\lt q$:
$$\sum_{n=0}^\infty \frac{x^{qn+p-1}}{qn+p}=-\frac{1}{q}\sum_{d=0}^{q-1} \frac{\omega_q^{(1-p)d}\ln(1-\omega_q^d x)}{\omega_q^d x}$$
Thus, it follows from this that
$$\sum_{n=0}^\infty \frac{x^{n}}{qn+p}=-\frac{x^{(1-p)/q}}{q}\sum_{d=0}^{q-1} \frac{\omega_q^{(1-p)d}\ln(1-\omega_q^d x^{1/q})}{\omega_q^d x^{1/q}}$$
and so, continuing the chain of equalities that I began earlier,
$$\begin{align}
\psi(p/q)
&= -\gamma+\lim_{x\to 1^-}\sum_{n=0}^\infty\frac{x^{n}}{n+1}-\frac{qx^{n}}{qn+p}\\
&= -\gamma+\lim_{x\to 1^-}\bigg[-\frac{\ln(1-x)}{x}+x^{(1-p)/q}\sum_{d=0}^{q-1} \frac{\omega_q^{(1-p)d}\ln(1-\omega_q^d x^{1/q})}{\omega_q^d x^{1/q}}\bigg]\\
&= -\gamma+\lim_{x\to 1^-}\bigg[-\frac{\ln(1-x)}{x}+x^{(1-p)/q}\ln(1-x^{1/q})+x^{(1-p)/q}\sum_{d=1}^{q-1} \frac{\omega_q^{(1-p)d}\ln(1-\omega_q^d x^{1/q})}{\omega_q^d x^{1/q}}\bigg]\\
&= -\gamma+\lim_{x\to 1^-}\bigg[-\frac{\ln(1-x)}{1}+1^{(1-p)/q}\ln(1-x^{1/q})+x^{(1-p)/q}\sum_{d=1}^{q-1} \frac{\omega_q^{(1-p)d}\ln(1-\omega_q^d x^{1/q})}{\omega_q^d x^{1/q}}\bigg]\\
&= -\gamma+\lim_{x\to 1^-}\bigg[-\ln(1-x)+\ln(1-x^{1/q})+x^{(1-p)/q}\sum_{d=1}^{q-1} \frac{\omega_q^{(1-p)d}\ln(1-\omega_q^d x^{1/q})}{\omega_q^d x^{1/q}}\bigg]\\
&= -\gamma+\lim_{x\to 1^-}\bigg[-\ln((1-x^{1/q})(1+x^{1/q}+x^{2/q}+...+x^{(q-1)/q}))+\ln(1-x^{1/q})+x^{(1-p)/q}\sum_{d=1}^{q-1} \frac{\omega_q^{(1-p)d}\ln(1-\omega_q^d x^{1/q})}{\omega_q^d x^{1/q}}\bigg]\\
&= -\gamma+\lim_{x\to 1^-}\bigg[-\ln(1+x^{1/q}+x^{2/q}+...+x^{(q-1)/q})+x^{(1-p)/q}\sum_{d=1}^{q-1} \frac{\omega_q^{(1-p)d}\ln(1-\omega_q^d x^{1/q})}{\omega_q^d x^{1/q}}\bigg]\\
&= -\gamma-\ln(1+1^{1/q}+1^{2/q}+...+1^{(q-1)/q})+\lim_{x\to 1^-}\bigg[x^{(1-p)/q}\sum_{d=1}^{q-1} \frac{\omega_q^{(1-p)d}\ln(1-\omega_q^d x^{1/q})}{\omega_q^d x^{1/q}}\bigg]\\
&= -\gamma-\ln(q)+\lim_{x\to 1^-}\bigg[x^{(1-p)/q}\sum_{d=1}^{q-1} \frac{\omega_q^{(1-p)d}\ln(1-\omega_q^d x^{1/q})}{\omega_q^d x^{1/q}}\bigg]\\
&= -\gamma-\ln(q)+\sum_{d=1}^{q-1} \frac{\omega_q^{(1-p)d}\ln(1-\omega_q^d)}{\omega_q^d}\\
&= -\gamma-\ln(q)+\sum_{d=1}^{q-1} \omega_q^{-pd}\ln(1-\omega_q^d)\\
\end{align}$$

Yuck, look at that nasty algebra. Just look away for a moment and take a little break. Here are a few more formulas that I am going to use in just a moment:
$$\ln(a+bi)=\frac{\ln(a^2+b^2)}{2}+i\arctan\frac{b}{a}$$
$$\cot \frac{x}{2}=\frac{\sin(x)}{1-\cos(x)}$$
$$2-2\cos(2x)=4\sin^2(x)$$
$$\arctan \cot x=\frac{\pi}{2}-x,\space\space\space x\in [0,\pi)$$
$$\sum_{d=1}^{q-1} \cos\frac{2\pi p d}{q}=-1,\space\space\space p,q\in\mathbb N$$
$$\sum_{d=1}^{q-1} \sin\frac{2\pi p d}{q}=0,\space\space\space p,q\in\mathbb N$$
$$\sum_{d=1}^{q-1} \frac{\pi d}{q}\sin\frac{2\pi p d}{q}=-\frac{\pi}{2}\cot\frac{\pi p}{q},\space\space\space p,q\in\mathbb N$$

These formulas are all pretty easy to derive, so I won't derive them for you. Keep an eye out for them as I continue the derivation - I'm not going to point them out.

Ready? Here we go.

$$\begin{align}
\psi(p/q)
&= -\gamma-\ln(q)+\sum_{d=1}^{q-1} \omega_q^{-pd}\ln(1-\omega_q^d)\\
&= -\gamma-\ln(q)+\sum_{d=1}^{q-1} \bigg(\cos \frac{2\pi pd}{q}-i\sin \frac{2\pi pd}{q}\bigg)\ln\bigg(1-\cos \frac{2\pi d}{q}-i\sin \frac{2\pi d}{q}\bigg)\\
&= -\gamma-\ln(q)+\sum_{d=1}^{q-1} \bigg(\cos \frac{2\pi pd}{q}-i\sin \frac{2\pi pd}{q}\bigg) \bigg(\frac{\ln((1-\cos(2\pi d/q))^2+\sin^2 (2\pi d/q))}{2}-i\arctan \frac{\sin(2\pi d/q)}{1-\cos(2\pi d/q)} \bigg)\\
&= -\gamma-\ln(q)+\sum_{d=1}^{q-1} \bigg(\cos \frac{2\pi pd}{q}-i\sin \frac{2\pi pd}{q}\bigg) \bigg(\frac{\ln(2-2\cos(2\pi d/q))}{2}-i\arctan \frac{\sin(2\pi d/q)}{1-\cos(2\pi d/q)} \bigg)\\
&= -\gamma-\ln(q)+\sum_{d=1}^{q-1} \bigg(\cos \frac{2\pi pd}{q}-i\sin \frac{2\pi pd}{q}\bigg) \bigg(\frac{\ln(4\sin^2(\pi d/q))}{2}-i\arctan \frac{\sin(2\pi d/q)}{1-\cos(2\pi d/q)} \bigg)\\
&= -\gamma-\ln(q)+\sum_{d=1}^{q-1} \bigg(\cos \frac{2\pi pd}{q}-i\sin \frac{2\pi pd}{q}\bigg) \bigg(\ln(2\sin(\pi d/q))-i\arctan \frac{\sin(2\pi d/q)}{1-\cos(2\pi d/q)} \bigg)\\
\end{align}$$
Because $\psi(p/q)$ is a real number for rational $p/q$, it follows that the right side of the equality is a real number, and so we may ignore the imaginary parts of each term of the summation, since they are guaranteed to cancel out to zero. Thus, we have
$$\begin{align}
\psi(p/q)
&= -\gamma-\ln(q)+\sum_{d=1}^{q-1} \Re\bigg[\bigg(\cos \frac{2\pi pd}{q}-i\sin \frac{2\pi pd}{q}\bigg) \bigg(\ln(2\sin(\pi d/q))-i\arctan \frac{\sin(2\pi d/q)}{1-\cos(2\pi d/q)} \bigg)\bigg]\\
&= -\gamma-\ln(q)+\sum_{d=1}^{q-1} \bigg(\cos \frac{2\pi pd}{q} \ln(2\sin(\pi d/q))-\sin \frac{2\pi pd}{q} \arctan \frac{\sin(2\pi d/q)}{1-\cos(2\pi d/q)}\bigg)\\
&= -\gamma-\ln(q)+\sum_{d=1}^{q-1} \bigg(\cos \frac{2\pi pd}{q} \ln(2\sin(\pi d/q))-\sin \frac{2\pi pd}{q} \arctan \cot\frac{\pi d}{q}\bigg)\\
&= -\gamma-\ln(q)+\sum_{d=1}^{q-1} \bigg(\cos \frac{2\pi pd}{q} \ln(2\sin(\pi d/q))-\sin \frac{2\pi pd}{q} \arctan \cot\frac{\pi d}{q}\bigg)\\
&= -\gamma-\ln(q)+\sum_{d=1}^{q-1}\cos \frac{2\pi pd}{q} \ln(2)+\sum_{d=1}^{q-1} \bigg(\cos \frac{2\pi pd}{q} \ln(\sin(\pi d/q))-\sin \frac{2\pi pd}{q} \arctan \cot\frac{\pi d}{q}\bigg)\\
&= -\gamma-\ln(q)-\ln(2)+\sum_{d=1}^{q-1} \bigg(\cos \frac{2\pi pd}{q} \ln(\sin(\pi d/q))-\sin \frac{2\pi pd}{q} \arctan \cot\frac{\pi d}{q}\bigg)\\
&= -\gamma-\ln(2q)+\sum_{d=1}^{q-1} \bigg(\cos \frac{2\pi pd}{q} \ln(\sin(\pi d/q))-\sin \frac{2\pi pd}{q} \bigg(\frac{\pi}{2}-\frac{\pi d}{q}\bigg)\bigg)\\
&= -\gamma-\ln(2q)+\sum_{d=1}^{q-1}\sin \frac{2\pi pd}{q} \bigg(\frac{\pi d}{q}-\frac{\pi}{2}\bigg)+\sum_{d=1}^{q-1} \bigg(\cos \frac{2\pi pd}{q} \ln(\sin(\pi d/q))\bigg)\\
&= -\gamma-\ln(2q)-\frac{\pi}{2}\cot\frac{\pi p}{q}+\sum_{d=1}^{q-1} \cos \frac{2\pi pd}{q} \ln \sin \frac{\pi d}{q}\\
\end{align}$$

This is it! This is the result we've been working towards!

$$\bbox[lightgray,5px]
{
\psi(p/q)= -\gamma-\ln(2q)-\frac{\pi}{2}\cot\frac{\pi p}{q}+\sum_{d=1}^{q-1} \cos \frac{2\pi pd}{q} \ln \sin \frac{\pi d}{q}
}$$

Of course, this only works for $p/q\in (0,1)$. However, if we want it to work for all rational numbers, we can simply use its recurrence
$$\psi(z+1)-\psi(z)=\frac{1}{z}$$
to say that

$$\psi(n+p/q)= -\gamma-\ln(2q)-\frac{\pi}{2}\cot\frac{\pi p}{q}+\sum_{d=1}^{q-1} \cos \frac{2\pi pd}{q} \ln \sin \frac{\pi d}{q}+\sum_{k=0}^{n-1} \frac{1}{k+\frac{p}{q}}$$

or

$$\psi(-n+p/q)= -\gamma-\ln(2q)-\frac{\pi}{2}\cot\frac{\pi p}{q}+\sum_{d=1}^{q-1} \cos \frac{2\pi pd}{q} \ln \sin \frac{\pi d}{q}+\sum_{k=0}^{n-1} \frac{1}{k-\frac{p}{q}}$$

Using these two formulas, it is easy to verify that, for any rational number $r$,

$$\psi(1-r)-\psi(r)=\pi\cos(\pi r)$$

Since the digamma function is continuous except at nonpositive integers, this property must necessarily extend to all *real* numbers, meaning that

$$\bbox[lightgray,5px]
{
\psi(1-z)-\psi(z)=\pi\cos(\pi z)
}$$

By integrating both sides of this with respect to $z$, we get
$$\ln\Gamma(1-z)+\ln\Gamma(z)=-\ln(\sin z)+C$$
By taking $z=1/2$, we can solve and obtain $C=\ln\pi$, giving us
$$\ln\Gamma(1-z)+\ln\Gamma(z)=-\ln(\sin z)+\ln\pi$$
and, by exponentiating both sides, we get the famous Gamma function reflection formula:
$$\bbox[lightgray,5px]
{
\Gamma(z)\Gamma(1-z)=\frac{\pi}{\sin(\pi z)}
}$$

I conclude this post with an exercise for the reader. Using this reflection formula, can you calculate the value of the following integral?

$$\int_0^1 \ln \Gamma(z)dz$$

**NOTE:** This is called **Raabe's Integral**, and the more general form
$$\int_a^{a+1} \ln \Gamma(z)dz$$
can also be evaluated.


